SP1Clean/Faithful/LtOperationSigned.lean
@@ -1,6 +1,6 @@
 import Mathlib.Tactic
 import Mathlib.Data.ZMod.Basic
-import SP1Clean.Operations.LtOperationSigned
+import SP1Clean.Operations.LtOperationSigned.RawSpec
 import SP1Clean.Foundations.SP1Constraint
 import SP1Clean.Extracted.LtOperationSigned
 import SP1Clean.Faithful.LtOperationUnsigned
